move to_simple_ruleset

SemanticsTernary/pfprefix_PF_To_Iptables.thy
@@ -380,40 +380,6 @@ fun pf_decision_to_ipt_decision :: "decision \<Rightarrow> state" where
 "pf_decision_to_ipt_decision decision.Accept = Decision FinalAllow" |
 "pf_decision_to_ipt_decision decision.Reject = Decision FinalDeny"
 
-definition to_simple_ruleset :: "'a line list \<Rightarrow> 'a line list" where
-"to_simple_ruleset rs = remove_quick_approx (remove_matches (remove_anchors' rs))"
-
-lemma
-  assumes "no_match_quick rs"
-      and "no_unknown_anchors (pfprefix_PrimitiveMatchers.common_matcher ctx, pfprefix_Unknown_Match_Tacs.in_doubt_allow) rs"
-  shows
- "pf_approx rs (pfprefix_PrimitiveMatchers.common_matcher ctx, pfprefix_Unknown_Match_Tacs.in_doubt_allow) p =
-  pf_approx (to_simple_ruleset rs) (pfprefix_PrimitiveMatchers.common_matcher ctx, pfprefix_Unknown_Match_Tacs.in_doubt_allow) p"
-  and "simple_ruleset (to_simple_ruleset rs)"
-proof(-)
-  have *: "(pf_approx rs (pfprefix_PrimitiveMatchers.common_matcher ctx, pfprefix_Unknown_Match_Tacs.in_doubt_allow) p) =
-        (pf_approx (remove_anchors' rs) (pfprefix_PrimitiveMatchers.common_matcher ctx, pfprefix_Unknown_Match_Tacs.in_doubt_allow) p)"
-    (is "?original = pf_approx (?anchors_removed) ?m ?p")
-    using assms by (simp add:remove_anchors'_preserves_semantics)
-  have na:"no_anchors ?anchors_removed" by (simp add:remove_anchors'_ok)
-  have nmq:"no_match_quick ?anchors_removed" using assms remove_anchors'_preserves_no_match_quick by blast
-  have *: "?original = pf_approx (remove_matches ?anchors_removed) ?m ?p"
-(is "?original = pf_approx (?matches_removed) ?m ?p")
-    using * na nmq assms by(auto simp add:remove_matches_preserves_semantics)
-  have nm:"no_match ?matches_removed" using na nmq remove_matches_ok by blast
-  have na:"no_anchors ?matches_removed" using na using remove_matches_preserves_no_anchors by blast
-  have gm:"good_matcher ?m" by (simp add:in_doubt_allow_good_matcher)
-  have *: "?original = pf_approx (remove_quick_approx ?matches_removed) ?m ?p"
-    (is "?original = pf_approx (?quick_removed) ?m ?p")
-    using * na nm gm assms by(simp add:remove_quick_approx_preserves_semantics)
-  then show "pf_approx rs (pfprefix_PrimitiveMatchers.common_matcher ctx, pfprefix_Unknown_Match_Tacs.in_doubt_allow) p =
-  pf_approx (to_simple_ruleset rs) (pfprefix_PrimitiveMatchers.common_matcher ctx, pfprefix_Unknown_Match_Tacs.in_doubt_allow) p" 
-    unfolding to_simple_ruleset_def by simp
-  have nq:"no_quick ?quick_removed" using na remove_quick_approx_ok by blast
-  have nm:"no_match ?quick_removed" using na nm remove_quick_approx_preserves_no_match by blast
-  have na:"no_anchors ?quick_removed" using na remove_quick_approx_preserves_no_anchors by blast
-  from nq nm na show "simple_ruleset (to_simple_ruleset rs)" unfolding to_simple_ruleset_def by (simp add:simple_ruleset_def)
-qed
 
 theorem
   assumes "no_match_quick rs"
